StepWf : coE, coD, col props

Coq/src/Step.v
@@ -91,14 +91,13 @@ Definition add_ew ews w' S S' : Prop :=
   ⟪ ewsEWprcl : dom_rel (ew S ⨾ ⦗ews⦘) ⊆₁ ews ⟫ /\
   ⟪ EW' : ew S' ≡ ew S ∪ ew_delta ews w' ⟫. 
 
-(* Do we really need `\₁ cf S' w'` part ??? *)
-Definition co_ws w' S S' := 
-  E S ∩₁ W S ∩₁ same_loc S' w' \₁ cf S' w'.
+Definition ws_compl ews ws S := 
+  codom_rel (⦗ews ∪₁ ws⦘ ⨾ co S) \₁ (ews ∪₁ ws).
 
 Definition co_delta ews ws w' S : relation eventid := 
-  ws × eq w' ∪ eq w' × (codom_rel (⦗ews ∪₁ ws⦘ ⨾ co S) \₁ (ews ∪₁ ws)).
+  ws × eq w' ∪ eq w' × ws_compl ews ws S.
 
-Hint Unfold co_ws co_delta : ESStepDb.
+Hint Unfold ws_compl co_delta : ESStepDb.
 
 Definition add_co ews ws w' S S' : Prop := 
   ⟪ wE' : E S' w' ⟫ /\
@@ -177,6 +176,52 @@ Definition hb_delta S S' k e e' : relation eventid :=
   (hb S)^? ⨾ (ESBasicStep.sb_delta S k e e' ∪ sw_delta S S' k e e') ⨾ (eq e × eq_opt e')^? . 
 
 Hint Unfold jfi_delta jfe_delta sw_delta hb_delta : ESStepDb.
+
+(******************************************************************************)
+(** ** ws_compl lemmas *)
+(******************************************************************************)
+
+Lemma ws_complE ews ws S 
+      (wf : ES.Wf S) : 
+  ws_compl ews ws S ⊆₁ E S.
+Proof. 
+  unfold ws_compl.
+  rewrite ES.coE; auto.
+  basic_solver.
+Qed.
+
+Lemma ws_complW ews ws S 
+      (wf : ES.Wf S) : 
+  ws_compl ews ws S ⊆₁ W S.
+Proof. 
+  unfold ws_compl.
+  rewrite ES.coD; auto.
+  basic_solver.
+Qed.
+
+Lemma ws_compl_loc ews ws w' e e' S S'
+      (wf : ES.Wf S) 
+      (BSTEP : ESBasicStep.t e e' S S') 
+      (AEW : add_ew ews w' S S')
+      (ACO : add_co ews ws w' S S') : 
+  ws_compl ews ws S ⊆₁ same_loc S' w'.
+Proof. 
+  cdes AEW; cdes ACO.
+  unfold ws_compl.
+  rewrite ES.coE; auto.
+  rewrite ewsLOC at 1.
+  rewrite wsLOC at 1.
+  rewrite ES.col; auto.
+  rewrite set_unionK.
+  intros x [[y HH] _].
+  unfolder in HH. desc.
+  etransitivity; eauto.
+  arewrite (loc S' y = loc S y).
+  { erewrite ESBasicStep.basic_step_loc_eq_dom; eauto. }
+  arewrite (loc S' x = loc S x).
+  { erewrite ESBasicStep.basic_step_loc_eq_dom; eauto. }
+  done. 
+Qed.
 
 (******************************************************************************)
 (** ** Deltas lemmas *)
@@ -1462,79 +1507,6 @@ Qed.
 (** ** Step (add_co) properties *)
 (******************************************************************************)
 
-(* we'll need this hack because of the way 
-     `loc` is defined in IMM *)
-Definition labloc lbl :=
-  match lbl with
-  | Aload _ _ l _
-  | Astore _ _ l _ => Some l
-  | _ => None
-  end.
-
-Lemma basic_step_co_ws_alt lang k k' st st' w' lbl e e' S S'
-      (BSTEP_ : ESBasicStep.t_ lang k k' st st' e e' S S') 
-      (wfE: ES.Wf S) 
-      (LBL : lab S' w' = lbl) 
-      (wEE' : (eq e ∪₁ eq_opt e') w') :
-  co_ws w' S S' ≡₁ E S ∩₁ W S ∩₁ (fun w => loc S w = labloc lbl) \₁ ES.cont_cf_dom S k.
-Proof. 
-  cdes BSTEP_.
-  assert (ESBasicStep.t e e' S S') as BSTEP.
-  { subst. econstructor. eauto. }
-
-  assert (
-    E S ∩₁ (same_loc S') w' ≡₁ E S ∩₁ (fun w : nat => (loc S) w = labloc lbl)
-  ) as LOCEQV.
-  { unfold Events.same_loc. 
-    unfolder; splits; intros x [Ex LOCx]; splits; auto.
-    { erewrite <- ESBasicStep.basic_step_loc_eq_dom; eauto.
-      rewrite <- LOCx. unfold Events.loc, labloc.
-      by rewrite LBL. }
-    erewrite ESBasicStep.basic_step_loc_eq_dom
-      with (x := x); eauto.
-    rewrite LOCx. unfold Events.loc, labloc.
-    by rewrite LBL. }
-
-  assert (
-    E S ∩₁ set_compl ((cf S') w') ≡₁ E S ∩₁ set_compl (ES.cont_cf_dom S k) 
-  ) as CFEQV.
-  { unfolder; splits; intros x [Ex nCFx]; splits; auto.
-    { intros nKCFx. apply nCFx.
-      eapply ESBasicStep.basic_step_cf; eauto.
-      autounfold with ESStepDb.
-      generalize wEE' nKCFx. 
-      basic_solver 10. }
-    assert (~ E S w') as nEw'.
-    { red. ins. destruct wEE' as [HA | HB]; desf.
-      { eapply ESBasicStep.basic_step_acts_set_ne; eauto. }
-      unfold eq_opt in HB. 
-      destruct e' as [e'|]; desf.
-      eapply ESBasicStep.basic_step_acts_set_ne'; eauto. }
-    intros CF. apply nCFx.    
-    eapply ESBasicStep.basic_step_cf in CF; eauto.
-    autounfold with ESStepDb in CF.
-    unfolder in CF. desf; exfalso.
-    { apply nEw'. apply ES.cfE, seq_eqv_lr in CF. desf. }
-    all : apply nEw'; eapply ES.cont_cf_domE in CF; eauto. }
-
-  unfold co_ws.
-
-  arewrite (
-    E S ∩₁ W S ∩₁ (same_loc S') w' \₁ (cf S') w' ≡₁
-      E S ∩₁ W S ∩₁ 
-        (E S ∩₁ (same_loc S') w') ∩₁ (E S \₁ (cf S') w')
-  ) by basic_solver.
-
-
-  arewrite (
-    E S ∩₁ W S ∩₁ (fun w : nat => (loc S) w = labloc lbl) \₁ ES.cont_cf_dom S k ≡₁
-    E S ∩₁ W S ∩₁ 
-      (E S ∩₁ (fun w : nat => (loc S) w = labloc lbl)) ∩₁ (E S \₁ ES.cont_cf_dom S k)
-  ) by basic_solver.
-
-  apply set_inter_Propere; auto.
-  apply set_inter_Propere; auto.
-Qed.
 
 (******************************************************************************)
 (** ** Step properties *)
